$V=\sum_i\frac{1}{2}m\omega_x^2\left[x_i^2+\left(\frac{\omega_y}{\omega_x}\right)^2y_i^2\right]+\sum_{i<j}\frac{e^2}{4\pi\epsilon_0\sqrt{(x_i-x_j)^2+(y_i-y_j)^2}}$
$\frac{V}{m\omega_x^2}=\sum_i\frac{1}{2}\left[x_i^2+\left(\frac{\omega_y}{\omega_x}\right)^2y_i^2\right]+\sum_{i<j}\frac{e^2}{4\pi\epsilon_0m\omega_x^2\sqrt{(x_i-x_j)^2+(y_i-y_j)^2}}$
To kill the dimension, we set $x_i=lu_i$, $y_i=lv_i$. Then we have
$\frac{V}{m\omega_x^2}=l^2\sum_i\frac{1}{2}\left[u_i^2+\left(\frac{\omega_y}{\omega_x}\right)^2v_i^2\right]+\frac{e^2}{4\pi\epsilon_0m\omega_x^2l}\sum_{i<j}\frac{1}{\sqrt{(u_i-u_j)^2+(v_i-v_j)^2}}$
If $l^2=\frac{e^2}{4\pi\epsilon_0m\omega_x^2l}$ we can have the dimensionless potential
Then let $l^3=\frac{e^2}{4\pi\epsilon_0m\omega_x^2}$ and $r=\frac{\omega_y}{\omega_x}$
We can make an dimensionless potential
\frac{V}{m\omega_x^2l^2}=\sum_i\frac{1}{2}\left(u_i^2+r^2v_i^2\right)+\sum_{i<j}\frac{1}{\sqrt{(u_i-u_j)^2+(v_i-v_j)^2}}
